start event marshaling proof

example/event.go
@@ -5,7 +5,7 @@ import (
 )
 
 type Event struct {
-	name  string
+	id    uint32
 	start TimeStamp
 	end   TimeStamp
 }
@@ -13,8 +13,8 @@ type Event struct {
 func MarshalEvent(e *Event) []byte {
 	// Getting the length right during code generation could be tricky
 	// How important is knowing the capacity in the first place?
-	var enc = make([]byte, 0, len(e.name)+24)
-	enc = marshal.WriteBytes(enc, []byte(e.name))
+	var enc = make([]byte, 0, 28)
+	enc = marshal.WriteInt32(enc, e.id)
 	enc = marshal.WriteBytes(enc, MarshalTimeStamp(&e.start))
 	enc = marshal.WriteBytes(enc, MarshalTimeStamp(&e.end))
 	return enc
@@ -23,10 +23,7 @@ func MarshalEvent(e *Event) []byte {
 func UnmarshalEvent(s []byte) *Event {
 	e := new(Event)
 	var enc = s // Needed for goose compatibility
-	var str_l uint64 = uint64(len(s) - 24)
-	var bytes []byte
-	bytes, enc = marshal.ReadBytes(enc, str_l)
-	e.name = string(bytes)
+	e.id, enc = marshal.ReadInt32(enc)
 	e.start = *UnmarshalTimeStamp(enc[:12])
 	enc = enc[12:]
 	e.end = *UnmarshalTimeStamp(enc[:12])
