example/main.go
@@ -10,13 +10,13 @@ func main() {
 	// This simple example creates a new event, then marshals and unmarshals it into
 	// a new Event before printing the result.
 
-	event := Event{name: "Grackle Meeting", start: TimeStamp{hour: 13, minute: 00, second: 00}, end: TimeStamp{hour: 14, minute: 00, second: 00}}
-	fmt.Printf("Name:  %v\nStart: %02d:%02d:%02d\nEnd:   %02d:%02d:%02d\n", event.name, event.start.hour, event.start.minute, event.start.second, event.end.hour, event.end.minute, event.end.second)
+	event := Event{id: 1, start: TimeStamp{hour: 13, minute: 00, second: 00}, end: TimeStamp{hour: 14, minute: 00, second: 00}}
+	fmt.Printf("Name:  %v\nStart: %02d:%02d:%02d\nEnd:   %02d:%02d:%02d\n", event.id, event.start.hour, event.start.minute, event.start.second, event.end.hour, event.end.minute, event.end.second)
 
 	enc := MarshalEvent(&event)
 
 	var newEvent *Event
 	newEvent = UnmarshalEvent(enc)
 
-	fmt.Printf("Name:  %v\nStart: %02d:%02d:%02d\nEnd:   %02d:%02d:%02d\n", newEvent.name, newEvent.start.hour, newEvent.start.minute, newEvent.start.second, newEvent.end.hour, newEvent.end.minute, newEvent.end.second)
+	fmt.Printf("Name:  %v\nStart: %02d:%02d:%02d\nEnd:   %02d:%02d:%02d\n", newEvent.id, newEvent.start.hour, newEvent.start.minute, newEvent.start.second, newEvent.end.hour, newEvent.end.minute, newEvent.end.second)
 }
