example/goose/example/example.v
@@ -6,10 +6,20 @@ Section code.
 Context `{ext_ty: ext_types}.
 Local Coercion Var' s: expr := Var s.
 
+(* event.go *)
+
+(* TimeStamp from timestamp.go *)
+
 Definition TimeStamp := struct.decl [
   "hour" :: uint32T;
   "minute" :: uint32T;
   "second" :: uint32T
+].
+
+Definition Event := struct.decl [
+  "id" :: uint32T;
+  "start" :: struct.t TimeStamp;
+  "end" :: struct.t TimeStamp
 ].
 
 Definition MarshalTimeStamp: val :=
@@ -18,6 +28,14 @@ Definition MarshalTimeStamp: val :=
     "enc" <-[slice.T byteT] (marshal.WriteInt32 (![slice.T byteT] "enc") (struct.loadF TimeStamp "hour" "t"));;
     "enc" <-[slice.T byteT] (marshal.WriteInt32 (![slice.T byteT] "enc") (struct.loadF TimeStamp "minute" "t"));;
     "enc" <-[slice.T byteT] (marshal.WriteInt32 (![slice.T byteT] "enc") (struct.loadF TimeStamp "second" "t"));;
+    ![slice.T byteT] "enc".
+
+Definition MarshalEvent: val :=
+  rec: "MarshalEvent" "e" :=
+    let: "enc" := ref_to (slice.T byteT) (NewSliceWithCap byteT #0 #28) in
+    "enc" <-[slice.T byteT] (marshal.WriteInt32 (![slice.T byteT] "enc") (struct.loadF Event "id" "e"));;
+    "enc" <-[slice.T byteT] (marshal.WriteBytes (![slice.T byteT] "enc") (MarshalTimeStamp (struct.fieldRef Event "start" "e")));;
+    "enc" <-[slice.T byteT] (marshal.WriteBytes (![slice.T byteT] "enc") (MarshalTimeStamp (struct.fieldRef Event "end" "e")));;
     ![slice.T byteT] "enc".
 
 Definition UnmarshalTimeStamp: val :=
@@ -34,5 +52,19 @@ Definition UnmarshalTimeStamp: val :=
     struct.storeF TimeStamp "second" "t" "0_ret";;
     "enc" <-[slice.T byteT] "1_ret";;
     "t".
+
+Definition UnmarshalEvent: val :=
+  rec: "UnmarshalEvent" "s" :=
+    let: "e" := struct.alloc Event (zero_val (struct.t Event)) in
+    let: "enc" := ref_to (slice.T byteT) "s" in
+    let: ("0_ret", "1_ret") := marshal.ReadInt32 (![slice.T byteT] "enc") in
+    struct.storeF Event "id" "e" "0_ret";;
+    "enc" <-[slice.T byteT] "1_ret";;
+    struct.storeF Event "start" "e" (struct.load TimeStamp (UnmarshalTimeStamp (SliceTake (![slice.T byteT] "enc") #12)));;
+    "enc" <-[slice.T byteT] (SliceSkip byteT (![slice.T byteT] "enc") #12);;
+    struct.storeF Event "end" "e" (struct.load TimeStamp (UnmarshalTimeStamp (SliceTake (![slice.T byteT] "enc") #12)));;
+    "e".
+
+(* timestamp.go *)
 
 End code.
