example/event_marshal_proof.v
@@ -1,0 +1,66 @@
+From Perennial.program_proof Require Import grove_prelude.
+From Grackle.example Require Import example.
+From Perennial.program_proof Require Import marshal_stateless_proof.
+From Grackle.example Require Import marshal_proof.
+
+Module encodeEvent.
+Section encodeEvent.
+
+Context `{!heapGS Σ}.
+
+Record EventStruct :=
+  mkC {
+      id : u32 ;
+      startTime : list u8 ;
+      endTime : list u8 ;
+    }.
+
+Definition has_encoding (encoded:list u8) (args:EventStruct) : Prop :=
+  encoded = (u32_le args.(id)) ++ args.(startTime) ++ args.(endTime).
+
+Definition own args_ptr args q : iProp Σ :=
+  ∃ start_sl end_sl,
+  "Hargs_id" ∷ args_ptr ↦[Event :: "id"]{q} #args.(id) ∗
+  "Hargs_start" ∷ args_ptr ↦[Event :: "startTime"]{q} (slice_val start_sl) ∗
+  "Hargs_start_sl" ∷ own_slice_small start_sl byteT q args.(startTime) ∗
+  "Hargs_end" ∷ args_ptr ↦[Event :: "endTime"]{q} (slice_val end_sl) ∗
+  "Hargs_end_sl" ∷ own_slice_small end_sl byteT q args.(endTime).
+
+Lemma wp_Encode (args_ptr:loc) (args:EventStruct) :
+  {{{
+        own args_ptr args (DfracDiscarded)
+  }}}
+    MarshalEvent #args_ptr
+  {{{
+        enc enc_sl, RET (slice_val enc_sl);
+        ⌜has_encoding enc args⌝ ∗
+        own_slice enc_sl byteT (DfracOwn 1) enc
+  }}}.
+Proof.
+  iIntros (?) "H HΦ". iNamed "H". wp_rec.
+  wp_apply (wp_NewSliceWithCap).
+  { apply encoding.unsigned_64_nonneg. }
+  iIntros (?) "Hsl".
+  wp_apply (wp_ref_to); first by val_ty.
+  iIntros (?) "Hptr".
+  wp_pures.
+
+  wp_loadField. wp_load. wp_apply (wp_WriteInt32 with "[$]").
+  iIntros (?) "Hsl". wp_store.
+
+  wp_apply (wp_struct_fieldRef_pointsto). { simpl. Admitted.
+
+Lemma wp_Decode enc enc_sl (args:EventStruct) :
+  {{{
+        ⌜has_encoding enc args⌝ ∗
+        own_slice_small enc_sl byteT (DfracOwn 1) enc
+  }}}
+    UnmarshalEvent (slice_val enc_sl)
+  {{{
+        args_ptr, RET #args_ptr; own args_ptr args (DfracOwn 1)
+  }}}.
+Proof.
+  Admitted.
+
+End encodeEvent.
+End encodeEvent.
